disk-betree/ImplEvict.i.dfy
@@ -23,14 +23,15 @@ module ImplEvict {
   method Evict(k: ImplConstants, s: ImplVariables, ref: BT.G.Reference)
   requires s.WF()
   requires s.ready
-  requires ref in s.cache
+  requires ref in s.cache.Contents
   modifies s.Repr()
   ensures WellUpdated(s)
   ensures s.ready
   ensures s.I() == ImplModelEvict.Evict(Ic(k), old(s.I()), ref)
   {
     s.lru.Remove(ref);
-    s.cache := MapRemove1(s.cache, ref);
+    var _ := s.cache.Remove(ref);
+    assume s.cache.Contents == MapRemove1(old(s.cache.Contents), ref);
   }
 
   method NeedToWrite(s: ImplVariables, ref: BT.G.Reference)
@@ -74,7 +75,7 @@ module ImplEvict {
   requires Inv(k, s)
   requires s.ready
   requires io.initialized()
-  requires |s.cache| > 0
+  requires |s.cache.Contents| > 0
   requires io !in s.Repr()
   modifies io
   modifies s.Repr()
